ulib/FStar.Monotonic.HyperHeap.fst
@@ -435,14 +435,6 @@ abstract val lemma_extends_fresh_disjoint: i:rid -> j:rid -> ipar:rid -> jpar:ri
          SMTPat (extends j jpar)]
 let lemma_extends_fresh_disjoint i j ipar jpar m0 m1 = ()
 
-let disjoint_regions (s1:Set.set rid) (s2:Set.set rid) =
-     forall x y. {:pattern (Set.mem x s1); (Set.mem y s2)} (Set.mem x s1 /\ Set.mem y s2) ==> disjoint x y
-
-let extends_parent (tip:rid{tip<>root}) (r:rid)
-  : Lemma (ensures (extends r (parent tip) /\ r<>tip ==> disjoint r tip \/ extends r tip))
-          [SMTPat (extends r (parent tip))]
-  = ()
-
 (*
 //  * AR: we can prove this lemma only if both the mreferences have same preorder
 //  *)
